editing ETCSN

ETCSIL.sml
@@ -1,4 +1,11 @@
 
+
+(*internal logic via truth table:
+
+Conj: T T
+DISJ
+
+*)
 val IMP_ex = prove_store("IMP_ex",
 e0
 (cheat)
@@ -6,10 +13,16 @@ e0
 “?imp: (1+1) * (1+1) -> 1+1. 
  !p1 p2. imp o Pa(p1,p2) = TRUE <=> (p1 = TRUE ==> p2 = TRUE)”));
 
-rastt "a:(1 + 1 ->A) o (imp : 2 * 2 -> 2)"
 
 
+(*
 
 val _ = new_fun "2" (ob_sort,[])
 
 val _ = new_abbr ("+",[ONE,ONE])  ("2",[]) 
+
+rastt "a:(1 + 1 ->A) o (imp : 2 * 2 -> 2)" problem
+
+need a function subst_ast which subst aId"2" into "1 + 1"
+
+*)
