ETCSind_tac.sml
@@ -1,0 +1,247 @@
+fun binop_t s t1 t2 = mk_fun s [t1,t2]
+
+fun unop_t s t = mk_fun s [t]
+
+val And = binop_t "And"
+
+val Or = binop_t "Or"
+
+val Imp = binop_t "Imp"
+
+val Iff = binop_t "Iff"
+
+val id = unop_t "id"
+
+val ALL = unop_t "ALL";
+
+val EX = unop_t "EX";
+
+val UE = unop_t "UE";
+
+fun dest_ar s = 
+    case view_sort s of
+       vSrt("ar",[d,c]) => (d,c) 
+     | _ => raise simple_fail "not an arr"
+
+val dom = fst o dest_ar 
+val cod = snd o dest_ar 
+
+fun bounds f = 
+    case view_form f of 
+        vQ(q,n,s,b) => (n,s) :: bounds b
+      | vConn(_,[f]) => bounds f
+      | vConn(_,[f1,f2]) => (bounds f1) @ (bounds f2)
+      | vPred _ => []
+      | vConn(_,l) => raise simple_fail "bounds.wrong input"
+
+fun Pol l = 
+    case l of 
+       [] => raise ERR ("Pol.empty input",[],[],[])
+      |h :: t => 
+       (case t of 
+           [] => h
+         | h1 :: t1 => 
+           (case t1 of 
+               [] => Po h h1
+             | h2 :: t2 => 
+               Po h (Pol t)))
+
+fun mk_pj n1 n2 =
+    mk_fun ("p" ^ (Int.toString n1) ^ (Int.toString n2))
+
+fun mk_pj n1 n2 =
+    if n1 = 1 andalso n2 = 1 then mk_fun "id" 
+    else if n1 = 2 andalso n2 = 1 then mk_fun "p1" 
+    else if n1 = 2 andalso n2 = 2 then mk_fun "p2"
+    else
+    mk_fun ("p" ^ (Int.toString n1) ^ (Int.toString n2))
+
+
+fun pos n l = 
+    case l of 
+        [] => raise simple_fail "pos.not a list member"
+      | h :: t => if h = n then 1 else (pos n t) + 1
+
+fun Pal l = 
+    case l of 
+       [] => raise ERR ("Pal.empty input",[],[],[])
+      |h :: t => 
+       (case t of 
+           [] =>  h
+         | h1 :: t1 => 
+           (case t1 of 
+               [] => Pa h h1
+             | h2 :: t2 => 
+               Pa h (Pal t)))
+
+
+(*fsym dict records the information that:
+Sub(n1,n2) should be SUB o Pa(n1,n2),
+so it does not build IL terms with Sub, but SUB.
+
+and hence not require the rw to expand the def of Sub to get distrib.
+
+only record the string and the term that the function symbol coressponds. Assuming they corresponds as uniform as:
+Sub(n1,n2) |-> SUB o Pa2(n1,n2)
+Same as Mul, Add, and for unary:
+
+Suc(n) |-> Suc o Pa1(n) (:= Suc o n)
+
+*)
+
+
+val fsym2IL0 = inserts (Binarymap.mkDict String.compare)
+[("Sub",mk_fun "SUB" []),("Suc",mk_fun "SUC" []),
+ ("Add",mk_fun "ADD" []),("Sub",mk_fun "SUB" [])]
+
+val fsym2IL = ref fsym2IL0
+
+fun new_fsym2IL (fsym,fterm) = 
+fsym2IL := Binarymap.insert(!fsym2IL,fsym,fterm)
+
+fun term2IL bvs t =
+    let val doms = List.map (cod o snd) bvs
+        val tn = length doms
+        val vdom = el tn doms
+    in
+        case view_term t of 
+            vVar(n,s) => 
+            if not $ mem (n,s) bvs then 
+               binop_t "o" t (unop_t "To1" (Pol doms))
+            else mk_pj tn (pos (n,s) bvs) doms
+          | vFun(f,s,tl) => 
+            if length tl = 0 then binop_t "o" t (unop_t "To1" (Pol doms))
+            else
+                let val args = List.map (term2IL bvs) tl
+                in
+                case Binarymap.peek(!fsym2IL,f) of 
+                    SOME fterm =>  binop_t "o" fterm (Pal args)
+                    (*(rewr_conv (spec_all th) t0) |> concl |> dest_eq |> #2*)
+                  | NONE => mk_fun f args
+                end
+          | _ => raise simple_fail "bound variables should not be here"
+    end;  
+
+
+
+
+val truth = mk_fun "TRUE" []
+
+
+fun mk_pred_ap pt args = (mk_o pt (Pal args))
+
+
+fun inserts d l = List.foldr (fn ((a,b),d) => Binarymap.insert(d,a,b)) d l
+
+
+val psym2IL0 = inserts (Binarymap.mkDict String.compare)
+[("IN",(rastt "Mem(X)",
+        [("x",ar_sort (mk_ob "A") (mk_ob "X")),
+         ("xs",ar_sort (mk_ob "A") (rastt "Exp(X,1+1)"))]))]
+(*
+[("Le",(rastt "Char(LE)",[])),
+ ("Lt",(rastt "Char(LT)",[])),(*
+ ("HasCard",(rastt "hasCard(X)",
+             [("xs",ar_sort (mk_ob "A") (rastt "Exp(X,1+1)")),
+              ("n",ar_sort (mk_ob "A") N)])),*)
+ ("Even",(rastt "EVEN",[])),
+ ("IN",(rastt "Mem(X)",
+        [("x",ar_sort (mk_ob "A") (mk_ob "X")),
+         ("xs",ar_sort (mk_ob "A") (rastt "Exp(X,1+1)"))])),
+ ("Sim",(rastt "relJ",[]))]
+*)
+
+val psym2IL = ref psym2IL0
+
+fun new_psym2IL (pred,(predfun,inputs)) = 
+psym2IL := Binarymap.insert(!psym2IL,pred,(predfun,inputs))
+
+(*
+form2IL [dest_var $ rastt "xs:1->Exp(X,1+1)",dest_var $ rastt "n:1->N"]
+“!x:1->K.HasCard(xs:1->Exp(X,1+1),n:1->N)” 
+keep this example
+
+*)
+
+
+val DISJ = mk_fun "DISJ" []
+
+val IFF = mk_fun "IFF" []
+
+val NEG = mk_fun "NEG" []
+
+fun binop_t s t1 t2 = mk_fun s [t1,t2]
+
+fun unop_t s t = mk_fun s [t]
+
+fun And p q = mk_o CONJ (Pa p q)
+
+fun Or p q = mk_o DISJ (Pa p q)
+
+fun Imp p q = mk_o IMP (Pa p q)
+
+fun Iff p q = mk_o IFF (Pa p q)
+
+fun Neg p = mk_o NEG p
+
+val id = unop_t "id"
+ 
+fun dest_cross AB = 
+    case view_term AB of 
+        vFun("*",_,[A,B]) => (A,B)
+      | _ => raise simple_fail "dest_cross.not a product"
+
+
+fun ALL f = 
+    let val d = dom (sort_of f)
+        val (X,Y) = dest_cross d
+    in mk_o (mk_fun "All" [X]) (Tp f)
+    end 
+
+
+fun EX f = 
+    let val d = dom (sort_of f)
+        val (X,Y) = dest_cross d
+    in mk_o (mk_fun "Ex" [X]) (Tp f)
+    end 
+
+
+fun UE f = 
+    let val d = dom (sort_of f)
+        val (X,Y) = dest_cross d
+    in mk_o (mk_fun "UE" [X]) (Tp f)
+    end 
+
+
+
+fun form2IL bvs f = 
+    case view_form f of 
+        vConn("&",[f1,f2]) => 
+        And (form2IL bvs f1) (form2IL bvs f2)
+      | vConn("|",[f1,f2]) => 
+        Or (form2IL bvs f1) (form2IL bvs f2)
+      | vConn("==>",[f1,f2]) => 
+        Imp (form2IL bvs f1) (form2IL bvs f2)
+      | vConn("<=>",[f1,f2]) => 
+        Iff (form2IL bvs f1) (form2IL bvs f2)
+      | vConn("~",[f0]) =>
+        Neg (form2IL bvs f0)
+      | vPred("=",true,[t1,t2]) =>
+        mk_pred_ap (mk_fun "Eq" [cod (sort_of t2)])
+         [term2IL bvs t1,term2IL bvs t2]
+      | vPred(P,_,tl) => 
+        (case Binarymap.peek(!psym2IL,P) of
+            SOME (p,l) => 
+            if l = []  then
+                mk_pred_ap p (List.map (term2IL bvs) tl)
+            else let val env = match_tl essps (List.map mk_var l) 
+                                        (List.map (term2IL bvs) tl) emptyvd
+                     in mk_pred_ap (inst_term env p) (List.map (term2IL bvs) tl)
+                 end
+          | _ => raise simple_fail ("form2IL.pred: " ^ P ^ " not found"))
+      | vQ ("!",n,s,b) => ALL (form2IL ((n,s) :: bvs) b)
+      | vQ ("?",n,s,b) => EX (form2IL ((n,s) :: bvs) b)
+      | vQ ("?!",n,s,b) => UE (form2IL ((n,s) :: bvs) b)
+      | _ => raise ERR ("form2IL.ill-formed formula",[],[],[f])
+
+
